tmc_lang -> lambda_lang. tmc_human_lang -> lambda_human_lang.

theories/tmc/definition.v
@@ -2,18 +2,18 @@ From simuliris Require Import
   prelude.
 From simuliris.common Require Export
   fin_maps.
-From simuliris.tmc_lang Require Export
+From simuliris.lambda_lang Require Export
   syntax.
-From simuliris.tmc_lang Require Import
+From simuliris.lambda_lang Require Import
   notations.
 
-Implicit Types func func_dps : function.
-Implicit Types v vₛ vₜ : val.
-Implicit Types e eₛ eₜ : expr.
-Implicit Types prog progₛ progₜ : program.
-Implicit Types ξ : gmap function function.
+Implicit Types func func_dps : lambda_function.
+Implicit Types v vₛ vₜ : lambda_val.
+Implicit Types e eₛ eₜ : lambda_expr.
+Implicit Types prog progₛ progₜ : lambda_program.
+Implicit Types ξ : gmap lambda_function lambda_function.
 
-Inductive tmc_dir ξ : expr → expr → Prop :=
+Inductive tmc_dir ξ : lambda_expr → lambda_expr → Prop :=
   | tmc_dir_val v :
       tmc_dir ξ
         #v
@@ -37,14 +37,14 @@ Inductive tmc_dir ξ : expr → expr → Prop :=
   | tmc_dir_unop op eₛ eₜ :
       tmc_dir ξ eₛ eₜ →
       tmc_dir ξ
-        (Unop op eₛ)
-        (Unop op eₜ)
+        (LambdaUnop op eₛ)
+        (LambdaUnop op eₜ)
   | tmc_dir_binop op eₛ1 eₛ2 eₜ1 eₜ2 :
       tmc_dir ξ eₛ1 eₜ1 →
       tmc_dir ξ eₛ2 eₜ2 →
       tmc_dir ξ
-        (Binop op eₛ1 eₛ2)
-        (Binop op eₜ1 eₜ2)
+        (LambdaBinop op eₛ1 eₛ2)
+        (LambdaBinop op eₜ1 eₜ2)
   | tmc_dir_if eₛ0 eₛ1 eₛ2 eₜ0 eₜ1 eₜ2 :
       tmc_dir ξ eₛ0 eₜ0 →
       tmc_dir ξ eₛ1 eₜ1 →
@@ -89,7 +89,7 @@ Inductive tmc_dir ξ : expr → expr → Prop :=
       tmc_dir ξ
         (eₛ1 <-[eₛ2]- eₛ3)
         (eₜ1 <-[eₜ2]- eₜ3)
-with tmc_dps ξ : expr → expr → expr → expr → Prop :=
+with tmc_dps ξ : lambda_expr → lambda_expr → lambda_expr → lambda_expr → Prop :=
   | tmc_dps_base dst idx eₛ eₜ :
       tmc_dir ξ eₛ eₜ →
       tmc_dps ξ dst idx
@@ -104,7 +104,7 @@ with tmc_dps ξ : expr → expr → expr → expr → Prop :=
   | tmc_dps_call dst idx func func_dps eₛ eₜ eₜ' :
       ξ !! func = Some func_dps →
       tmc_dir ξ eₛ eₜ →
-      eₜ' = (let: eₜ in func_dps (dst.[ren (+1)], idx.[ren (+1)], $0))%E →
+      eₜ' = (let: eₜ in func_dps (dst.[ren (+1)], idx.[ren (+1)], $0))%lambda_expr →
       tmc_dps ξ dst idx
         (func eₛ)
         eₜ'
@@ -118,14 +118,14 @@ with tmc_dps ξ : expr → expr → expr → expr → Prop :=
   | tmc_dps_constr_1 dst idx constr eₛ1 eₛ2 eₜ1 eₜ2 eₜ :
       tmc_dir ξ eₛ1 eₜ1 →
       tmc_dps ξ $0 𝟚 eₛ2.[ren (+1)] eₜ2 →
-      eₜ = (let: &constr eₜ1 #() in dst.[ren (+1)] <-[idx.[ren (+1)]]- $0 ;; eₜ2)%E →
+      eₜ = (let: &constr eₜ1 #() in dst.[ren (+1)] <-[idx.[ren (+1)]]- $0 ;; eₜ2)%lambda_expr →
       tmc_dps ξ dst idx
         (&constr eₛ1 eₛ2)
         eₜ
   | tmc_dps_constr_2 dst idx constr eₛ1 eₛ2 eₜ1 eₜ2 eₜ :
       tmc_dir ξ eₛ2 eₜ2 →
       tmc_dps ξ $0 𝟙 eₛ1.[ren (+1)] eₜ1 →
-      eₜ = (let: &constr #() eₜ2 in dst.[ren (+1)] <-[idx.[ren (+1)]]- $0 ;; eₜ1)%E →
+      eₜ = (let: &constr #() eₜ2 in dst.[ren (+1)] <-[idx.[ren (+1)]]- $0 ;; eₜ1)%lambda_expr →
       tmc_dps ξ dst idx
         (&constr eₛ1 eₛ2)
         eₜ.
@@ -140,7 +140,7 @@ Create HintDb tmc.
 #[export] Hint Constructors tmc_dps : tmc.
 
 Record tmc {progₛ progₜ} := {
-  tmc_ξ : gmap function function ;
+  tmc_ξ : gmap lambda_function lambda_function ;
 
   tmc_ξ_dom :
     dom tmc_ξ ⊆ dom progₛ ;
@@ -162,6 +162,6 @@ Record tmc {progₛ progₜ} := {
         let: ![𝟙] $1 in
         let: ![𝟚] $3 in
         eₜ
-      )%E ;
+      )%lambda_expr ;
 }.
 #[global] Arguments tmc : clear implicits.
