theories/tmc/examples/list_append.v
@@ -1,15 +1,15 @@
 From simuliris Require Import
   prelude.
-From simuliris.tmc_lang Require Export
+From simuliris.lambda_lang Require Export
   refinement.
-From simuliris.tmc_human_lang Require Export
+From simuliris.lambda_human_lang Require Export
   compilation.
-From simuliris.tmc_human_lang Require Import
+From simuliris.lambda_human_lang Require Import
   notations.
 From simuliris.tmc Require Import
   soundness.
 
-Definition list_append : human_program := {[
+Definition list_append : lambda_human_program := {[
   "list_append" := (BNamed "arg", (
     let: "xs" := ![𝟙] "arg" in
     let: "ys" := ![𝟚] "arg" in
@@ -19,10 +19,10 @@ Definition list_append : human_program := {[
     | CONS "x", "xs" =>
         CONSₕ "x" ($"list_append" ("xs", "ys"))
     end
-  )%HE)
+  )%lambda_human_expr)
 ]}.
 
-Definition list_append_tmc : human_program := {[
+Definition list_append_tmc : lambda_human_program := {[
   "list_append" := (BNamed "arg", (
     let: "xs" := ![𝟙] "arg" in
     let: "ys" := ![𝟚] "arg" in
@@ -36,7 +36,7 @@ Definition list_append_tmc : human_program := {[
         ) ;;
         "dst"
     end
-  )%HE) ;
+  )%lambda_human_expr) ;
   "list_append_dps" := (BNamed "arg", (
     let: "dst_idx" := ![𝟙] "arg" in
     let: "idx" := ![𝟚] "dst_idx" in
@@ -53,21 +53,21 @@ Definition list_append_tmc : human_program := {[
         let: "arg" := ("xs", "ys") in
         $"list_append_dps" ("dst'", 𝟚, "arg")
     end
-  )%HE)
+  )%lambda_human_expr)
 ]}.
 
 Lemma list_append_tmc_sound :
-  program_refinement
-    (human_program_compile list_append)
-    (human_program_compile list_append_tmc).
+  lambda_program_refinement
+    (lambda_human_program_compile list_append)
+    (lambda_human_program_compile list_append_tmc).
 Proof.
   rewrite /list_append /list_append_tmc. apply tmc_sound.
   - split.
-    + apply human_program_compile_well_formed.
-      rewrite /human_program_well_formed map_Forall_singleton //.
-    + rewrite /human_program_compile map_fmap_singleton /=.
-      rewrite /program_closed map_Forall_singleton. naive_solver lia.
-  - rewrite /human_program_compile map_fmap_singleton fmap_insert map_fmap_singleton /=.
+    + apply lambda_human_program_compile_well_formed.
+      rewrite /lambda_human_program_well_formed map_Forall_singleton //.
+    + rewrite /lambda_human_program_compile map_fmap_singleton /=.
+      rewrite /lambda_program_closed map_Forall_singleton. naive_solver lia.
+  - rewrite /lambda_human_program_compile map_fmap_singleton fmap_insert map_fmap_singleton /=.
     exists {["list_append" := "list_append_dps"]}; try set_solver.
     + intros * (<- & <-)%lookup_singleton_Some.
       rewrite lookup_insert.
