theories/common/three.v
@@ -1,0 +1,30 @@
+From stdpp Require Import
+  countable.
+
+From simuliris Require Import
+  prelude.
+
+Inductive three :=
+  | Zero
+  | One
+  | Two.
+
+#[global] Instance three_eq_dec : EqDecision three :=
+  ltac:(solve_decision).
+#[global] Instance three_countable :
+  Countable three.
+Proof.
+  pose encode idx :=
+    match idx with
+    | Zero => 0
+    | One => 1
+    | Two => 2
+    end.
+  pose decode idx :=
+    match idx with
+    | 0 => Zero
+    | 1 => One
+    | _ => Two
+    end.
+  apply (inj_countable' encode decode). intros []; done.
+Qed.
