theories/lambda_human_lang/compilation.v
@@ -1,0 +1,107 @@
+From simuliris Require Import
+  prelude.
+From simuliris.lambda_lang Require Export
+  well_formed.
+From simuliris.lambda_lang Require Import
+  notations.
+From simuliris.lambda_human_lang Require Export
+  well_formed.
+
+Definition lambda_human_bindings := list binder.
+Implicit Types bdgs : lambda_human_bindings.
+
+Fixpoint lambda_human_bindings_lookup_aux i bdgs x :=
+  match bdgs with
+  | [] =>
+      None
+  | y :: bdgs =>
+      if bool_decide (y = BNamed x)
+      then Some i
+      else lambda_human_bindings_lookup_aux (S i) bdgs x
+  end.
+Definition lambda_human_bindings_lookup bdgs x :=
+  lambda_human_bindings_lookup_aux 0 bdgs x.
+
+Definition lambda_human_val_compile v :=
+  match v with
+  | LambdaHumanUnit =>
+      LambdaUnit
+  | LambdaHumanIndex idx =>
+      LambdaIndex idx
+  | LambdaHumanInt n =>
+      LambdaInt n
+  | LambdaHumanBool b =>
+      LambdaBool b
+  | LambdaHumanFunc func =>
+      LambdaFunc func
+  end.
+
+Fixpoint lambda_human_expr_compile bdgs e :=
+  match e with
+  | LambdaHumanVal v =>
+      LambdaVal (lambda_human_val_compile v)
+  | LambdaHumanVar x =>
+      from_option LambdaVar Fail%lambda_expr (lambda_human_bindings_lookup bdgs x)
+  | LambdaHumanLet x e1 e2 =>
+      LambdaLet
+        (lambda_human_expr_compile bdgs e1)
+        (lambda_human_expr_compile (x :: bdgs) e2)
+  | LambdaHumanCall e1 e2 =>
+      LambdaCall
+        (lambda_human_expr_compile bdgs e1)
+        (lambda_human_expr_compile bdgs e2)
+  | LambdaHumanUnop op e =>
+      LambdaUnop op
+        (lambda_human_expr_compile bdgs e)
+  | LambdaHumanBinop op e1 e2 =>
+      LambdaBinop op
+        (lambda_human_expr_compile bdgs e1)
+        (lambda_human_expr_compile bdgs e2)
+  | LambdaHumanIf e0 e1 e2 =>
+      LambdaIf
+        (lambda_human_expr_compile bdgs e0)
+        (lambda_human_expr_compile bdgs e1)
+        (lambda_human_expr_compile bdgs e2)
+  | LambdaHumanConstr constr e1 e2 =>
+      LambdaConstr constr
+        (lambda_human_expr_compile bdgs e1)
+        (lambda_human_expr_compile bdgs e2)
+  | LambdaHumanLoad e1 e2 =>
+      LambdaLoad
+        (lambda_human_expr_compile bdgs e1)
+        (lambda_human_expr_compile bdgs e2)
+  | LambdaHumanStore e1 e2 e3 =>
+      LambdaStore
+        (lambda_human_expr_compile bdgs e1)
+        (lambda_human_expr_compile bdgs e2)
+        (lambda_human_expr_compile bdgs e3)
+  end.
+
+Definition lambda_human_program_compile (prog : lambda_human_program) : lambda_program :=
+  (λ '(x, e), lambda_human_expr_compile [x] e) <$> prog.
+
+Lemma lambda_human_val_compile_well_formed prog v :
+  lambda_human_program_well_formed prog →
+  lambda_human_val_well_formed prog v →
+  lambda_val_well_formed (lambda_human_program_compile prog) (lambda_human_val_compile v).
+Proof.
+  intros Hprog Hv. destruct v; try done. rewrite /= dom_fmap_L //.
+Qed.
+Lemma lambda_human_expr_compile_well_formed prog e bdgs :
+  lambda_human_program_well_formed prog →
+  lambda_human_expr_well_formed prog e →
+  lambda_expr_well_formed (lambda_human_program_compile prog) (lambda_human_expr_compile bdgs e).
+Proof.
+  intros Hprog He. revert bdgs. induction e; intros bdgs; try naive_solver; simpl.
+  - apply lambda_human_val_compile_well_formed; done.
+  - destruct (lambda_human_bindings_lookup bdgs _); done.
+Qed.
+Lemma lambda_human_program_compile_well_formed prog :
+  lambda_human_program_well_formed prog →
+  lambda_program_well_formed (lambda_human_program_compile prog).
+Proof.
+  intros Hprog. apply map_Forall_lookup.
+  intros func e ((x & he) & <- & Hfunc)%lookup_fmap_Some.
+  apply lambda_human_expr_compile_well_formed; first done.
+  rewrite /lambda_human_program_well_formed map_Forall_lookup in Hprog. naive_solver.
+Qed.
