theories/lambda_human_lang/notations.v
@@ -1,0 +1,127 @@
+From simuliris Require Import
+  prelude.
+From simuliris.lambda_lang Require Export
+  notations.
+From simuliris.lambda_human_lang Require Export
+  syntax.
+
+Coercion LambdaHumanIndex : lambda_index >-> lambda_human_val.
+Coercion LambdaHumanInt : Z >-> lambda_human_val.
+Coercion LambdaHumanBool : bool >-> lambda_human_val.
+
+Coercion LambdaHumanVal : lambda_human_val >-> lambda_human_expr.
+Coercion LambdaHumanVar : lambda_human_name >-> lambda_human_expr.
+Coercion LambdaHumanCall : lambda_human_expr >-> Funclass.
+
+Declare Scope lambda_human_val_scope.
+Delimit Scope lambda_human_val_scope with lambda_human_val.
+Bind Scope lambda_human_val_scope with lambda_human_val.
+
+Notation "()" := LambdaHumanUnit
+: lambda_human_val_scope.
+
+Declare Scope lambda_human_expr_scope.
+Delimit Scope lambda_human_expr_scope with lambda_human_expr.
+Bind Scope lambda_human_expr_scope with lambda_human_expr.
+
+Notation "#ₕ v" := (LambdaHumanVal v%Z%lambda_human_val%stdpp)
+( at level 5,
+  format "#ₕ v"
+).
+
+Notation "'Fail'" := (#ₕ() #ₕ())%lambda_human_expr
+: lambda_human_expr_scope.
+
+Notation "$ x" := (LambdaHumanFunc x)
+( at level 5,
+  format "$ x"
+) : lambda_human_expr_scope.
+
+Notation "'let:' x := e1 'in' e2" := (LambdaHumanLet x%binder e1%lambda_human_expr e2%lambda_human_expr)
+( at level 200,
+  x at level 1,
+  e1, e2 at level 200,
+  format "'[v' 'let:'  x  :=  '[' e1 ']'  'in' '/' e2 ']'"
+) : lambda_human_expr_scope.
+Notation "e1 ;; e2" := (LambdaHumanLet BAnon e1%lambda_human_expr e2%lambda_human_expr)
+( at level 100,
+  e2 at level 200,
+  format "'[v' '[hv' '[' e1 ']'  ;; ']' '/' e2 ']'"
+) : lambda_human_expr_scope.
+
+Notation "~ e" := (LambdaHumanUnop LambdaOpNeg e%lambda_human_expr)
+: lambda_human_expr_scope.
+Notation "- e" := (LambdaHumanUnop LambdaOpUminus e%lambda_human_expr)
+: lambda_human_expr_scope.
+
+Notation "e1 + e2" := (LambdaHumanBinop LambdaOpPlus e1%lambda_human_expr e2%lambda_human_expr)
+: lambda_human_expr_scope.
+Notation "e1 - e2" := (LambdaHumanBinop LambdaOpMinus e1%lambda_human_expr e2%lambda_human_expr)
+: lambda_human_expr_scope.
+Notation "e1 * e2" := (LambdaHumanBinop LambdaOpMult e1%lambda_human_expr e2%lambda_human_expr)
+: lambda_human_expr_scope.
+Notation "e1 `quot` e2" := (LambdaHumanBinop LambdaOpQuot e1%lambda_human_expr e2%lambda_human_expr)
+: lambda_human_expr_scope.
+Notation "e1 `rem` e2" := (LambdaHumanBinop LambdaOpRem e1%lambda_human_expr e2%lambda_human_expr)
+: lambda_human_expr_scope.
+Notation "e1 ≤ e2" := (LambdaHumanBinop LambdaOpLe e1%lambda_human_expr e2%lambda_human_expr)
+: lambda_human_expr_scope.
+Notation "e1 < e2" := (LambdaHumanBinop LambdaOpLt e1%lambda_human_expr e2%lambda_human_expr)
+: lambda_human_expr_scope.
+Notation "e1 = e2" := (LambdaHumanBinop LambdaOpEq e1%lambda_human_expr e2%lambda_human_expr)
+: lambda_human_expr_scope.
+Notation "e1 ≠ e2" := (~ (e1 = e2))%lambda_human_expr
+: lambda_human_expr_scope.
+
+Notation "'if:' e0 'then' e1 'else' e2" := (LambdaHumanIf e0%lambda_human_expr e1%lambda_human_expr e2%lambda_human_expr)
+( at level 200,
+  e0, e1, e2 at level 200
+) : lambda_human_expr_scope.
+Notation "e1 && e2" := (if: e1 then e2 else #ₕfalse)%lambda_human_expr
+( only parsing
+) : lambda_human_expr_scope.
+Notation "e1 || e2" := (if: e1 then #ₕtrue else e2)%lambda_human_expr
+( only parsing
+) : lambda_human_expr_scope.
+
+Notation "& constr" := (LambdaHumanConstr constr)
+( at level 5,
+  format "& constr"
+) : lambda_human_expr_scope.
+
+Notation "![ e2 ] e1" := (LambdaHumanLoad e1%lambda_human_expr e2%lambda_human_expr)
+( at level 9,
+  right associativity,
+  format "![ e2 ]  e1"
+) : lambda_human_expr_scope.
+Notation "! e" := (LambdaHumanLoad e%lambda_human_expr 𝟘)
+( at level 9,
+  right associativity,
+  format "! e"
+) : lambda_human_expr_scope.
+
+Notation "e1 <-[ e2 ]- e3" := (LambdaHumanStore e1%lambda_human_expr e2%lambda_human_expr e3%lambda_human_expr)
+( at level 20,
+  format "e1  <-[ e2 ]-  e3"
+) : lambda_human_expr_scope.
+
+Notation "( e1 , e2 , .. , en )" := (&CONSTR_PAIR .. (&CONSTR_PAIR e1 e2) .. en)%lambda_human_expr
+: lambda_human_expr_scope.
+
+Notation NILₕ := (&CONSTR_NIL #ₕ() #ₕ())%lambda_human_expr (only parsing).
+Notation CONSₕ := (&CONSTR_CONS)%lambda_human_expr (only parsing).
+Notation HEADₕ e := (![𝟙] e)%lambda_human_expr (only parsing).
+Notation TAILₕ e := (![𝟚] e)%lambda_human_expr (only parsing).
+Notation "'match:' e0 'with' 'NIL' => e1 | 'CONS' x , y => e2 'end'" := (
+  let: "__match" := e0 in
+  if: !"__match" = #ₕ(Z.of_nat CONSTR_NIL) then (
+    e1
+  ) else (
+    let: y := TAILₕ "__match" in
+    let: x := HEADₕ "__match" in
+    e2
+  )
+)%lambda_human_expr (
+  only parsing,
+  e0, e1, x, y, e2 at level 200
+) : lambda_human_expr_scope.
