theories/lambda_lang/language.v
@@ -1,0 +1,94 @@
+From simuliris Require Import
+  prelude.
+From simuliris.common Require Import
+  tactics.
+From simuliris.program_logic Require Export
+  ectxi_language.
+From simuliris.lambda_lang Require Export
+  semantics.
+
+Implicit Types l : loc.
+Implicit Types v w : lambda_val.
+Implicit Types e : lambda_expr.
+Implicit Types σ : lambda_state.
+
+Notation lambda_of_val := LambdaVal.
+
+Definition lambda_to_val e :=
+  match e with
+  | LambdaVal v => Some v
+  | _ => None
+  end.
+
+Canonical lambda_val_O := leibnizO lambda_val.
+Canonical lambda_expr_O := leibnizO lambda_expr.
+Canonical lambda_state_O := leibnizO lambda_state.
+
+Inductive lambda_ectxi :=
+  | LambdaEctxiLet e2
+  | LambdaEctxiCall1 e1
+  | LambdaEctxiCall2 v2
+  | LambdaEctxiUnop (op : lambda_unop)
+  | LambdaEctxiBinop1 (op : lambda_binop) e1
+  | LambdaEctxiBinop2 (op : lambda_binop) v2
+  | LambdaEctxiIf e1 e2
+  | LambdaEctxiLoad1 e1
+  | LambdaEctxiLoad2 v2
+  | LambdaEctxiStore1 e1 e2
+  | LambdaEctxiStore2 e1 v3
+  | LambdaEctxiStore3 v2 v3.
+
+Definition lambda_ectx := list lambda_ectxi.
+
+Definition lambda_fill_item k e :=
+  match k with
+  | LambdaEctxiLet e2 =>
+      LambdaLet e e2
+  | LambdaEctxiCall1 e1 =>
+      LambdaCall e1 e
+  | LambdaEctxiCall2 v2 =>
+      LambdaCall e (lambda_of_val v2)
+  | LambdaEctxiUnop op =>
+      LambdaUnop op e
+  | LambdaEctxiBinop1 op e1 =>
+      LambdaBinop op e1 e
+  | LambdaEctxiBinop2 op v2 =>
+      LambdaBinop op e (lambda_of_val v2)
+  | LambdaEctxiIf e1 e2 =>
+      LambdaIf e e1 e2
+  | LambdaEctxiLoad1 e1 =>
+      LambdaLoad e1 e
+  | LambdaEctxiLoad2 v2 =>
+      LambdaLoad e (lambda_of_val v2)
+  | LambdaEctxiStore1 e1 e2 =>
+      LambdaStore e1 e2 e
+  | LambdaEctxiStore2 e1 v3 =>
+      LambdaStore e1 e (lambda_of_val v3)
+  | LambdaEctxiStore3 v2 v3 =>
+      LambdaStore e (lambda_of_val v2) (lambda_of_val v3)
+  end.
+#[global] Instance lambda_ectxi_fill : Fill lambda_ectxi lambda_expr :=
+  Build_Fill lambda_fill_item.
+
+Lemma lambda_ectxi_lang_mixin :
+  EctxiLanguageMixin
+    lambda_of_val
+    lambda_to_val
+    lambda_head_step
+    lambda_ectxi.
+Proof.
+  split.
+  - naive_solver.
+  - intros []; naive_solver.
+  - intros * []; naive_solver.
+  - intros [] ?**; naive_solver.
+  - intros []; naive_solver.
+  - intros [] ? []; naive_solver.
+  - intros ? [] * Hstep; invert Hstep; naive_solver.
+Qed.
+Canonical lambda_ectxi_lang :=
+  Build_ectxi_language lambda_ectxi_lang_mixin.
+Canonical lambda_ectx_lang :=
+  ectx_language_of_ectxi_language lambda_ectxi_lang.
+Canonical lambda_lang :=
+  language_of_ectx_language lambda_ectx_lang.
