theories/lambda_lang/semantics.v
@@ -1,0 +1,151 @@
+From simuliris Require Import
+  prelude.
+From simuliris.lambda_lang Require Export
+  syntax.
+From simuliris.lambda_lang Require Import
+  notations.
+
+Definition lambda_state := gmap loc lambda_val.
+
+#[global] Instance lambda_state_eq_dec :
+  EqDecision lambda_state.
+Proof.
+  solve_decision.
+Defined.
+#[global] Instance lambda_state_inhabited :
+  Inhabited lambda_state.
+Proof.
+  apply _.
+Qed.
+
+Implicit Types b : bool.
+Implicit Types l : loc.
+Implicit Types func : lambda_function.
+Implicit Types constr : lambda_constructor.
+Implicit Types idx : lambda_index.
+Implicit Types v w : lambda_val.
+Implicit Types e : lambda_expr.
+Implicit Types prog : lambda_program.
+Implicit Types σ : lambda_state.
+
+Definition lambda_unop_eval op v :=
+  match op, v with
+  | LambdaOpNeg, LambdaBool b =>
+      Some (LambdaBool (negb b))
+  | LambdaOpUminus, LambdaInt n =>
+      Some (LambdaInt (- n))
+  | _, _ =>
+      None
+  end.
+
+Definition lambda_binop_eval_int op n1 n2 :=
+  match op with
+  | LambdaOpPlus =>
+      Some (LambdaInt (n1 + n2))
+  | LambdaOpMinus =>
+      Some (LambdaInt (n1 - n2))
+  | LambdaOpMult =>
+      Some (LambdaInt (n1 * n2))
+  | LambdaOpQuot =>
+      Some (LambdaInt (n1 `quot` n2))
+  | LambdaOpRem =>
+      Some (LambdaInt (n1 `rem` n2))
+  | LambdaOpLe =>
+      Some (LambdaBool (bool_decide (n1 ≤ n2)%Z))
+  | LambdaOpLt =>
+      Some (LambdaBool (bool_decide (n1 < n2)%Z))
+  | LambdaOpEq =>
+      Some (LambdaBool (bool_decide (n1 = n2)%Z))
+  end.
+Definition lambda_binop_eval_bool op b1 b2 :=
+  match op with
+  | LambdaOpEq =>
+      Some (LambdaBool (bool_decide (b1 = b2)))
+  | _ =>
+      None
+  end.
+Definition lambda_binop_eval_function op func1 func2 :=
+  match op with
+  | LambdaOpEq =>
+      Some (LambdaBool (bool_decide (func1 = func2)))
+  | _ =>
+      None
+  end.
+Definition lambda_binop_eval op v1 v2 :=
+  match v1, v2 with
+  | LambdaInt n1, LambdaInt n2 =>
+      lambda_binop_eval_int op n1 n2
+  | LambdaBool b1, LambdaBool b2 =>
+      lambda_binop_eval_bool op b1 b2
+  | LambdaFunc func1, LambdaFunc func2 =>
+      lambda_binop_eval_function op func1 func2
+  | _, _ =>
+      None
+  end.
+
+Inductive lambda_head_step prog : lambda_expr → lambda_state → lambda_expr → lambda_state → Prop :=
+  | lambda_head_step_let v e e' σ :
+      e' = e.[#v/] →
+      lambda_head_step prog
+        (let: v in e) σ
+        e' σ
+  | lambda_head_step_call func v e e' σ :
+      prog !! func = Some e →
+      e' = e.[#v/] →
+      lambda_head_step prog
+        (func v) σ
+        e' σ
+  | lambda_head_step_lambda_unop op v v' σ :
+      lambda_unop_eval op v = Some v' →
+      lambda_head_step prog
+        (LambdaUnop op v) σ
+        v' σ
+  | lambda_head_step_lambda_binop op v1 v2 v' σ :
+      lambda_binop_eval op v1 v2 = Some v' →
+      lambda_head_step prog
+        (LambdaBinop op v1 v2) σ
+        v' σ
+  | lambda_head_step_if b e1 e2 σ :
+      lambda_head_step prog
+        (if: b then e1 else e2) σ
+        (if b then e1 else e2) σ
+  | lambda_head_step_constr_1 constr e1 e2 e' σ :
+      e' = (let: e1 in let: e2.[ren (+1)] in &&constr $1 $0)%lambda_expr →
+      lambda_head_step prog
+        (&constr e1 e2) σ
+        e' σ
+  | lambda_head_step_constr_2 constr e1 e2 e' σ :
+      e' = (let: e2 in let: e1.[ren (+1)] in &&constr $0 $1)%lambda_expr →
+      lambda_head_step prog
+        (&constr e1 e2) σ
+        e' σ
+  | lambda_head_step_constr_det constr v1 v2 σ l :
+      σ !! (l +ₗ 0) = None →
+      σ !! (l +ₗ 1) = None →
+      σ !! (l +ₗ 2) = None →
+      lambda_head_step prog
+        (&&constr v1 v2) σ
+        l (<[l +ₗ 2 := v2]> (<[l +ₗ 1 := v1]> (<[l +ₗ 0 := LambdaInt (Z.of_nat constr)]> σ)))
+  | lambda_head_step_load l l' idx v σ :
+      σ !! (l +ₗ idx) = Some v →
+      lambda_head_step prog
+        (![idx] l) σ
+        v σ
+  | lambda_head_step_store l idx v w σ :
+      σ !! (l +ₗ idx) = Some v →
+      lambda_head_step prog
+        (l <-[idx]- w) σ
+        #() (<[l +ₗ idx := w]> σ).
+
+Lemma lambda_head_step_constr_det' prog constr v1 v2 σ σ' :
+  let l := loc_fresh (dom σ) in
+  σ' = <[l +ₗ 2 := v2]> (<[l +ₗ 1 := v1]> (<[l +ₗ 0 := LambdaInt (Z.of_nat constr)]> σ)) →
+  lambda_head_step prog
+    (&&constr v1 v2) σ
+    l σ'.
+Proof.
+  intros l ->.
+  apply lambda_head_step_constr_det;
+    rewrite -not_elem_of_dom;
+    apply loc_fresh_fresh; lia.
+Qed.
