theories/lambda_lang/syntax.v
@@ -1,0 +1,223 @@
+From stdpp Require Export
+  strings
+  gmap.
+From stdpp Require Import
+  countable.
+
+From simuliris Require Import
+  prelude.
+From simuliris.common Require Export
+  autosubst
+  three
+  loc
+  typeclasses.
+
+Notation lambda_function := string (only parsing).
+
+Definition lambda_constructor := nat.
+
+Notation lambda_index := three (only parsing).
+
+Inductive lambda_val :=
+  | LambdaUnit
+  | LambdaIndex (idx : lambda_index)
+  | LambdaInt (n : Z)
+  | LambdaBool (b : bool)
+  | LambdaLoc (l : loc)
+  | LambdaFunc (func : lambda_function).
+
+#[global] Instance lambda_val_inhabited : Inhabited lambda_val :=
+  populate LambdaUnit.
+#[global] Instance lambda_val_eq_dec : EqDecision lambda_val :=
+  ltac:(solve_decision).
+#[global] Instance lambda_val_countable :
+  Countable lambda_val.
+Proof.
+  pose encode v :=
+    match v with
+    | LambdaUnit =>
+        inl ()
+    | LambdaIndex idx =>
+        inr $ inl idx
+    | LambdaInt n =>
+        inr $ inr $ inl n
+    | LambdaBool b =>
+        inr $ inr $ inr $ inl b
+    | LambdaLoc l =>
+        inr $ inr $ inr $ inr $ inl l
+    | LambdaFunc func =>
+        inr $ inr $ inr $ inr $ inr func
+    end.
+  pose decode v :=
+    match v with
+    | inl () =>
+        LambdaUnit
+    | inr (inl idx) =>
+        LambdaIndex idx
+    | inr (inr (inl n)) =>
+        LambdaInt n
+    | inr (inr (inr (inl b))) =>
+        LambdaBool b
+    | inr (inr (inr (inr (inl l)))) =>
+        LambdaLoc l
+    | inr (inr (inr (inr (inr func)))) =>
+        LambdaFunc func
+    end.
+  apply (inj_countable' encode decode). intros []; done.
+Qed.
+
+#[global] Instance lambda_val_similar : Similar lambda_val lambda_val :=
+  Build_Similar $ λ v1 v2,
+    match v1, v2 with
+    | LambdaUnit, LambdaUnit =>
+        True
+    | LambdaIndex idx1, LambdaIndex idx2 =>
+        idx1 = idx2
+    | LambdaInt i1, LambdaInt i2 =>
+        i1 = i2
+    | LambdaBool b1, LambdaBool b2 =>
+        b1 = b2
+    | LambdaLoc _, LambdaLoc _ =>
+        True
+    | LambdaFunc func1, LambdaFunc func2 =>
+        func1 = func2
+    | _, _ =>
+        False
+    end.
+
+Inductive lambda_unop :=
+  | LambdaOpNeg | LambdaOpUminus.
+
+#[global] Instance lambda_unop_eq_dec : EqDecision lambda_unop :=
+  ltac:(solve_decision).
+#[global] Instance lambda_unop_countable :
+  Countable lambda_unop.
+Proof.
+  pose encode op :=
+    match op with
+    | LambdaOpNeg => 0
+    | LambdaOpUminus => 1
+    end.
+  pose decode op :=
+    match op with
+    | 0 => LambdaOpNeg
+    | _ => LambdaOpUminus
+    end.
+  apply (inj_countable' encode decode). intros []; done.
+Qed.
+
+Inductive lambda_binop :=
+  | LambdaOpPlus | LambdaOpMinus | LambdaOpMult | LambdaOpQuot | LambdaOpRem
+  | LambdaOpLe | LambdaOpLt | LambdaOpEq.
+
+#[global] Instance lambda_binop_eq_dec : EqDecision lambda_binop :=
+  ltac:(solve_decision).
+#[global] Instance lambda_binop_countable :
+  Countable lambda_binop.
+Proof.
+  pose encode op :=
+    match op with
+    | LambdaOpPlus => 0
+    | LambdaOpMinus => 1
+    | LambdaOpMult => 2
+    | LambdaOpQuot => 3
+    | LambdaOpRem => 4
+    | LambdaOpLe => 5
+    | LambdaOpLt => 6
+    | LambdaOpEq => 7
+    end.
+  pose decode op :=
+    match op with
+    | 0 => LambdaOpPlus
+    | 1 => LambdaOpMinus
+    | 2 => LambdaOpMult
+    | 3 => LambdaOpQuot
+    | 4 => LambdaOpRem
+    | 5 => LambdaOpLe
+    | 6 => LambdaOpLt
+    | _ => LambdaOpEq
+    end.
+  apply (inj_countable' encode decode). intros []; done.
+Qed.
+
+Inductive lambda_expr :=
+  | LambdaVal (v : lambda_val)
+  | LambdaVar (x : var)
+  | LambdaLet (e1 : lambda_expr) (e2 : {bind lambda_expr})
+  | LambdaCall (e1 e2 : lambda_expr)
+  | LambdaUnop (op : lambda_unop) (e : lambda_expr)
+  | LambdaBinop (op : lambda_binop) (e1 e2 : lambda_expr)
+  | LambdaIf (e0 e1 e2 : lambda_expr)
+  | LambdaConstr (constr : lambda_constructor) (e1 e2 : lambda_expr)
+  | LambdaConstrDet (constr : lambda_constructor) (e1 e2 : lambda_expr)
+  | LambdaLoad (e1 e2 : lambda_expr)
+  | LambdaStore (e1 e2 e3 : lambda_expr).
+
+#[global] Instance lambda_expr_inhabited : Inhabited lambda_expr :=
+  populate (LambdaVal inhabitant).
+#[global] Instance lambda_expr_eq_dec : EqDecision lambda_expr :=
+  ltac:(solve_decision).
+#[global] Instance lambda_expr_countable :
+  Countable lambda_expr.
+Proof.
+  pose fix encode e :=
+    match e with
+    | LambdaVal v =>
+        GenLeaf (inl v)
+    | LambdaVar x =>
+        GenLeaf (inr $ inl x)
+    | LambdaLet e1 e2 =>
+        GenNode 0 [encode e1; encode e2]
+    | LambdaCall e1 e2 =>
+        GenNode 1 [encode e1; encode e2]
+    | LambdaUnop op e =>
+        GenNode 2 [GenLeaf (inr $ inr $ inl op); encode e]
+    | LambdaBinop op e1 e2 =>
+        GenNode 3 [GenLeaf (inr $ inr $ inr $ inl op); encode e1; encode e2]
+    | LambdaIf e0 e1 e2 =>
+        GenNode 4 [encode e0; encode e1; encode e2]
+    | LambdaConstr constr e1 e2 =>
+        GenNode 5 [GenLeaf (inr $ inr $ inr $ inr constr); encode e1; encode e2]
+    | LambdaConstrDet constr e1 e2 =>
+        GenNode 6 [GenLeaf (inr $ inr $ inr $ inr constr); encode e1; encode e2]
+    | LambdaLoad e1 e2 =>
+        GenNode 7 [encode e1; encode e2]
+    | LambdaStore e1 e2 e3 =>
+        GenNode 8 [encode e1; encode e2; encode e3]
+    end.
+  pose fix decode e :=
+    match e with
+    | GenLeaf (inl v) =>
+        LambdaVal v
+    | GenLeaf (inr (inl x)) =>
+        LambdaVar x
+    | GenNode 0 [e1; e2] =>
+        LambdaLet (decode e1) (decode e2)
+    | GenNode 1 [e1; e2] =>
+        LambdaCall (decode e1) (decode e2)
+    | GenNode 2 [GenLeaf (inr (inr (inl op))); e] =>
+        LambdaUnop op (decode e)
+    | GenNode 3 [GenLeaf (inr (inr (inr (inl op)))); e1; e2] =>
+        LambdaBinop op (decode e1) (decode e2)
+    | GenNode 4 [e0; e1; e2] =>
+        LambdaIf (decode e0) (decode e1) (decode e2)
+    | GenNode 5 [GenLeaf (inr (inr (inr (inr constr)))); e1; e2] =>
+        LambdaConstr constr (decode e1) (decode e2)
+    | GenNode 6 [GenLeaf (inr (inr (inr (inr constr)))); e1; e2] =>
+        LambdaConstrDet constr (decode e1) (decode e2)
+    | GenNode 7 [e1; e2] =>
+        LambdaLoad (decode e1) (decode e2)
+    | GenNode 8 [e1; e2; e3] =>
+        LambdaStore (decode e1) (decode e2) (decode e3)
+    | _ =>
+        @inhabitant _ lambda_expr_inhabited
+    end.
+  apply (inj_countable' encode decode). intros e. induction e; simpl; congruence.
+Qed.
+
+#[global] Instance lambda_expr_ids : Ids lambda_expr. derive. Defined.
+#[global] Instance lambda_expr_rename : Rename lambda_expr. derive. Defined.
+#[global] Instance lambda_expr_subst : Subst lambda_expr. derive. Defined.
+#[global] Instance lambda_expr_subst_lemmas : SubstLemmas lambda_expr. derive. Qed.
+
+Definition lambda_program := gmap lambda_function lambda_expr.
