theories/lambda_lang/well_formed.v
@@ -1,0 +1,224 @@
+From simuliris Require Import
+  prelude.
+From simuliris.lambda_lang Require Export
+  syntax.
+
+Implicit Types prog : lambda_program.
+
+Definition lambda_val_well_formed prog v :=
+  match v with
+  | LambdaLoc _ =>
+      False
+  | LambdaFunc func =>
+      func ∈ dom prog
+  | _ =>
+      True
+  end.
+
+Fixpoint lambda_expr_well_formed prog e :=
+  match e with
+  | LambdaVal v =>
+      lambda_val_well_formed prog v
+  | LambdaVar _ =>
+      True
+  | LambdaLet e1 e2 =>
+      lambda_expr_well_formed prog e1 ∧
+      lambda_expr_well_formed prog e2
+  | LambdaCall e1 e2 =>
+      lambda_expr_well_formed prog e1 ∧
+      lambda_expr_well_formed prog e2
+  | LambdaUnop _ e =>
+      lambda_expr_well_formed prog e
+  | LambdaBinop _ e1 e2 =>
+      lambda_expr_well_formed prog e1 ∧
+      lambda_expr_well_formed prog e2
+  | LambdaIf e0 e1 e2 =>
+      lambda_expr_well_formed prog e0 ∧
+      lambda_expr_well_formed prog e1 ∧
+      lambda_expr_well_formed prog e2
+  | LambdaConstr _ e1 e2 =>
+      lambda_expr_well_formed prog e1 ∧
+      lambda_expr_well_formed prog e2
+  | LambdaConstrDet _ _ _ =>
+      False
+  | LambdaLoad e1 e2 =>
+      lambda_expr_well_formed prog e1 ∧
+      lambda_expr_well_formed prog e2
+  | LambdaStore e1 e2 e3 =>
+      lambda_expr_well_formed prog e1 ∧
+      lambda_expr_well_formed prog e2 ∧
+      lambda_expr_well_formed prog e3
+  end.
+
+Fixpoint lambda_expr_closed lvl e :=
+  match e with
+  | LambdaVal _ =>
+      True
+  | LambdaVar x =>
+      x < lvl
+  | LambdaLet e1 e2 =>
+      lambda_expr_closed lvl e1 ∧
+      lambda_expr_closed (S lvl) e2
+  | LambdaCall e1 e2 =>
+      lambda_expr_closed lvl e1 ∧
+      lambda_expr_closed lvl e2
+  | LambdaUnop _ e =>
+      lambda_expr_closed lvl e
+  | LambdaBinop _ e1 e2 =>
+      lambda_expr_closed lvl e1 ∧
+      lambda_expr_closed lvl e2
+  | LambdaIf e0 e1 e2 =>
+      lambda_expr_closed lvl e0 ∧
+      lambda_expr_closed lvl e1 ∧
+      lambda_expr_closed lvl e2
+  | LambdaConstr _ e1 e2 =>
+      lambda_expr_closed lvl e1 ∧
+      lambda_expr_closed lvl e2
+  | LambdaConstrDet _ _ _ =>
+      False
+  | LambdaLoad e1 e2 =>
+      lambda_expr_closed lvl e1 ∧
+      lambda_expr_closed lvl e2
+  | LambdaStore e1 e2 e3 =>
+      lambda_expr_closed lvl e1 ∧
+      lambda_expr_closed lvl e2 ∧
+      lambda_expr_closed lvl e3
+  end.
+
+Definition lambda_program_well_formed prog :=
+  map_Forall (λ _, lambda_expr_well_formed prog) prog.
+
+Definition lambda_program_closed prog :=
+  map_Forall (λ _, lambda_expr_closed 1) prog.
+
+Definition lambda_program_valid prog :=
+  lambda_program_well_formed prog ∧ lambda_program_closed prog.
+
+Lemma subst_lambda_expr_closed ς1 ς2 lvl e :
+  (∀ x, x < lvl → ς1 x = ς2 x) →
+  lambda_expr_closed lvl e →
+  e.[ς1] = e.[ς2].
+Proof.
+  revert ς1 ς2 lvl. induction e as
+    [ v
+    | x
+    | e1 IHe1 e2 IHe2
+    | e1 IHe1 e2 IHe2
+    | e IHe
+    | e1 IHe1 e2 IHe2
+    | e0 IHe0 e1 IHe1 e2 IHe2
+    | e1 IHe1 e2 IHe2
+    | e1 IHe1 e2 IHe2
+    | e1 IHe1 e2 IHe2
+    | e1 IHe1 e2 IHe2 e3 IHe3
+    ];
+    intros ς1 ς2 lvl Hς Hclosed;
+    asimpl;
+    try (f_equal; naive_solver).
+  f_equal; first naive_solver.
+  eapply IHe2; last naive_solver.
+  intros x Hx. destruct x; first done. asimpl. f_equal. naive_solver lia.
+Qed.
+Lemma subst_lambda_expr_closed_0 ς1 ς2 e :
+  lambda_expr_closed 0 e →
+  e.[ς1] = e.[ς2].
+Proof.
+  intros Hclosed.
+  eapply subst_lambda_expr_closed; last done.
+  lia.
+Qed.
+Lemma subst_lambda_expr_closed_1 ς1 ς2 e :
+  ς1 0 = ς2 0 →
+  lambda_expr_closed 1 e →
+  e.[ς1] = e.[ς2].
+Proof.
+  intros Hς Hclosed.
+  eapply subst_lambda_expr_closed; last done.
+  setoid_rewrite Nat.lt_1_r. naive_solver.
+Qed.
+Lemma subst_lambda_expr_closed_1' ς1 ς2 v e :
+  lambda_expr_closed 1 e →
+  e.[v .: ς1] = e.[v .: ς2].
+Proof.
+  apply subst_lambda_expr_closed_1. done.
+Qed.
+
+Lemma subst_lambda_program_closed ς1 ς2 prog func e :
+  ς1 0 = ς2 0 →
+  lambda_program_closed prog →
+  prog !! func = Some e →
+  e.[ς1] = e.[ς2].
+Proof.
+  intros Hσ Hwf Hlookup.
+  eapply subst_lambda_expr_closed_1; first done.
+  eapply map_Forall_lookup_1 in Hwf; naive_solver.
+Qed.
+Lemma subst_lambda_program_closed' ς1 ς2 v prog func e :
+  lambda_program_closed prog →
+  prog !! func = Some e →
+  e.[v .: ς1] = e.[v .: ς2].
+Proof.
+  apply subst_lambda_program_closed. done.
+Qed.
+
+Lemma lambda_expr_closed_le lvl1 lvl2 e :
+  lvl1 ≤ lvl2 →
+  lambda_expr_closed lvl1 e →
+  lambda_expr_closed lvl2 e.
+Proof.
+  revert lvl1 lvl2. elim e; try naive_solver lia.
+  intros e1 IH1 e2 IH2 lvl1 lvl2 Hlvl (Hclosed1 & Hclosed2).
+  split; first naive_solver. eapply IH2; last done. lia.
+Qed.
+
+Lemma lambda_expr_closed_upn_subst_lambda_val n v lvl e :
+  n < lvl →
+  lambda_expr_closed lvl e →
+  lambda_expr_closed (lvl - 1) e.[upn n (LambdaVal v .: ids)].
+Proof.
+  revert n lvl. induction e; intros n lvl; try naive_solver; simpl.
+  - intros Hn Hx.
+    destruct (Nat.lt_ge_cases x n) as [Hx' | (dx & ->)%Nat.le_sum].
+    + rewrite upn_lt //=. lia.
+    + rewrite upn_ge; first lia.
+      rewrite Nat.sub_add'. destruct dx; first done. simpl. lia.
+  - intros Hn (Hclosed1 & Hclosed2). split; first naive_solver.
+    rewrite fold_up_upn.
+    destruct lvl; first lia.
+    rewrite /= Nat.sub_0_r -(Nat.pred_succ (S lvl)) -Nat.sub_1_r.
+    auto with lia.
+Qed.
+Lemma lambda_expr_closed_subst_lambda_val lvl e v :
+  lambda_expr_closed lvl e →
+  lambda_expr_closed (lvl - 1) e.[LambdaVal v/].
+Proof.
+  destruct lvl.
+  - intros Hclosed%(lambda_expr_closed_le _ 1)%(lambda_expr_closed_upn_subst_lambda_val 0 v); naive_solver lia.
+  - apply (lambda_expr_closed_upn_subst_lambda_val 0). lia.
+Qed.
+
+Lemma lambda_expr_closed_ren ξ n lvl e :
+  (∀ x, ξ x ≤ x + n) →
+  lambda_expr_closed lvl e →
+  lambda_expr_closed (lvl + n) e.[ren ξ].
+Proof.
+  revert lvl ξ n. elim e; try naive_solver lia.
+  - intros x lvl ξ n Hξ Hclosed.
+    eapply (Nat.le_lt_trans _ (x + n)); naive_solver lia.
+  - intros e1 IH1 e2 IH2 lvl ξ n Hξ (Hclosed1 & Hclosed2).
+    split; first naive_solver.
+    asimpl. rewrite -Nat.add_succ_l. apply IH2; last done.
+    intros []; simpl; [lia | rewrite -Nat.succ_le_mono //].
+Qed.
+Lemma lambda_expr_closed_lift n lvl e :
+  lambda_expr_closed lvl e →
+  lambda_expr_closed (lvl + n) e.[ren (+n)].
+Proof.
+  apply lambda_expr_closed_ren. naive_solver lia.
+Qed.
+Lemma lambda_expr_closed_lift1 lvl e :
+  lambda_expr_closed lvl e →
+  lambda_expr_closed (S lvl) e.[ren (+1)].
+Proof.
+  rewrite -Nat.add_1_r. apply lambda_expr_closed_lift.
+Qed.
